some basic components for context pruning

ocaml/fstar-lib/generated/FStar_Extraction_ML_Modul.ml
@@ -2669,7 +2669,9 @@ and (extract_sig_let :
                      FStar_TypeChecker_Env.core_check =
                        (env.FStar_TypeChecker_Env.core_check);
                      FStar_TypeChecker_Env.missing_decl =
-                       (env.FStar_TypeChecker_Env.missing_decl)
+                       (env.FStar_TypeChecker_Env.missing_decl);
+                     FStar_TypeChecker_Env.pending_lemmas =
+                       (env.FStar_TypeChecker_Env.pending_lemmas)
                    } in
                  let lbd =
                    let uu___3 =
