ocaml/fstar-lib/generated/FStar_Interactive_Legacy.ml
@@ -147,7 +147,9 @@ let (push_with_kind :
               FStar_TypeChecker_Env.core_check =
                 (env.FStar_TypeChecker_Env.core_check);
               FStar_TypeChecker_Env.missing_decl =
-                (env.FStar_TypeChecker_Env.missing_decl)
+                (env.FStar_TypeChecker_Env.missing_decl);
+              FStar_TypeChecker_Env.pending_lemmas =
+                (env.FStar_TypeChecker_Env.pending_lemmas)
             } in
           let res = FStar_TypeChecker_Tc.push_context env1 msg in
           FStar_Options.push ();
