ocaml/fstar-lib/generated/FStar_Tactics_Hooks.ml
@@ -954,7 +954,9 @@ let rec (traverse_for_spinoff :
                              FStar_TypeChecker_Env.core_check =
                                (env2.FStar_TypeChecker_Env.core_check);
                              FStar_TypeChecker_Env.missing_decl =
-                               (env2.FStar_TypeChecker_Env.missing_decl)
+                               (env2.FStar_TypeChecker_Env.missing_decl);
+                             FStar_TypeChecker_Env.pending_lemmas =
+                               (env2.FStar_TypeChecker_Env.pending_lemmas)
                            } e1 in
                        (match uu___4 with
                         | (e2, lc) ->
@@ -1971,7 +1973,10 @@ let (splice :
                                          FStar_TypeChecker_Env.core_check =
                                            (env.FStar_TypeChecker_Env.core_check);
                                          FStar_TypeChecker_Env.missing_decl =
-                                           (env.FStar_TypeChecker_Env.missing_decl)
+                                           (env.FStar_TypeChecker_Env.missing_decl);
+                                         FStar_TypeChecker_Env.pending_lemmas
+                                           =
+                                           (env.FStar_TypeChecker_Env.pending_lemmas)
                                        }, val_t)
                                       (FStar_Syntax_Embeddings.e_tuple3
                                          (FStar_Syntax_Embeddings.e_list
