ocaml/fstar-lib/generated/FStar_TypeChecker_Env.ml
@@ -131,6 +131,92 @@ let (uu___is_DefaultUnivsToZero : step -> Prims.bool) =
   fun projectee ->
     match projectee with | DefaultUnivsToZero -> true | uu___ -> false
 type steps = step Prims.list
+type lemma_triggers = FStar_Ident.lident Prims.list Prims.list Prims.list
+type pending_lemma_patterns =
+  {
+  pending_lemma_triggers: lemma_triggers FStar_Compiler_Util.psmap ;
+  lidents_to_pending_lemmas:
+    FStar_Ident.lident Prims.list FStar_Compiler_Util.psmap }
+let (__proj__Mkpending_lemma_patterns__item__pending_lemma_triggers :
+  pending_lemma_patterns -> lemma_triggers FStar_Compiler_Util.psmap) =
+  fun projectee ->
+    match projectee with
+    | { pending_lemma_triggers; lidents_to_pending_lemmas;_} ->
+        pending_lemma_triggers
+let (__proj__Mkpending_lemma_patterns__item__lidents_to_pending_lemmas :
+  pending_lemma_patterns ->
+    FStar_Ident.lident Prims.list FStar_Compiler_Util.psmap)
+  =
+  fun projectee ->
+    match projectee with
+    | { pending_lemma_triggers; lidents_to_pending_lemmas;_} ->
+        lidents_to_pending_lemmas
+let (empty_pending_lemma_patterns : pending_lemma_patterns) =
+  let uu___ = FStar_Compiler_Util.psmap_empty () in
+  let uu___1 = FStar_Compiler_Util.psmap_empty () in
+  { pending_lemma_triggers = uu___; lidents_to_pending_lemmas = uu___1 }
+let (remove_pending_lemma :
+  FStar_Ident.lident -> pending_lemma_patterns -> pending_lemma_patterns) =
+  fun lid ->
+    fun p ->
+      let lid_str = FStar_Ident.string_of_lid lid in
+      let pending_lemmas =
+        FStar_Compiler_Util.psmap_remove p.lidents_to_pending_lemmas lid_str in
+      {
+        pending_lemma_triggers = (p.pending_lemma_triggers);
+        lidents_to_pending_lemmas = pending_lemmas
+      }
+let (remove_trigger_for_lemma :
+  FStar_Ident.lident ->
+    FStar_Ident.lident ->
+      pending_lemma_patterns -> (pending_lemma_patterns * Prims.bool))
+  =
+  fun pat ->
+    fun lem ->
+      fun ctxt ->
+        let pat_str = FStar_Ident.string_of_lid pat in
+        let lem_str = FStar_Ident.string_of_lid lem in
+        let pending_triggers_for_lem =
+          FStar_Compiler_Util.psmap_try_find ctxt.pending_lemma_triggers
+            lem_str in
+        match pending_triggers_for_lem with
+        | FStar_Pervasives_Native.None -> (ctxt, false)
+        | FStar_Pervasives_Native.Some triggers ->
+            let triggers1 =
+              FStar_Compiler_List.map
+                (fun disjunct ->
+                   FStar_Compiler_List.map
+                     (fun conjunct ->
+                        FStar_Compiler_List.filter
+                          (fun x ->
+                             let uu___ = FStar_Ident.string_of_lid x in
+                             uu___ <> pat_str) conjunct) disjunct) triggers in
+            let eligible =
+              FStar_Compiler_Util.for_some
+                (fun disjunct ->
+                   FStar_Compiler_List.for_all
+                     (fun conjunct -> Prims.uu___is_Nil conjunct) disjunct)
+                triggers1 in
+            let pending_lemma_triggers =
+              FStar_Compiler_Util.psmap_add ctxt.pending_lemma_triggers
+                lem_str triggers1 in
+            ({
+               pending_lemma_triggers;
+               lidents_to_pending_lemmas = (ctxt.lidents_to_pending_lemmas)
+             }, eligible)
+let (find_lemmas_waiting_on_trigger :
+  FStar_Ident.lident ->
+    pending_lemma_patterns -> FStar_Ident.lident Prims.list)
+  =
+  fun lid ->
+    fun ctxt ->
+      let lid_str = FStar_Ident.string_of_lid lid in
+      let uu___ =
+        FStar_Compiler_Util.psmap_try_find ctxt.lidents_to_pending_lemmas
+          lid_str in
+      match uu___ with
+      | FStar_Pervasives_Native.None -> []
+      | FStar_Pervasives_Native.Some lems -> lems
 let (dbg_ImplicitTrace : Prims.bool FStar_Compiler_Effect.ref) =
   FStar_Compiler_Debug.get_toggle "ImplicitTrace"
 let (dbg_LayeredEffectsEqns : Prims.bool FStar_Compiler_Effect.ref) =
@@ -478,7 +564,8 @@ and env =
             (FStar_Syntax_Syntax.typ FStar_Pervasives_Native.option,
               Prims.bool -> Prims.string) FStar_Pervasives.either
     ;
-  missing_decl: FStar_Ident.lident FStar_Compiler_RBSet.t }
+  missing_decl: FStar_Ident.lident FStar_Compiler_RBSet.t ;
+  pending_lemmas: pending_lemma_patterns }
 and solver_t =
   {
   init: env -> unit ;
@@ -611,8 +698,8 @@ let (__proj__Mkenv__item__solver : env -> solver_t) =
         fv_delta_depths; proof_ns; synth_hook; try_solve_implicits_hook;
         splice; mpreprocess; postprocess; identifier_info; tc_hooks; 
         dsenv; nbe; strict_args_tab; erasable_types_tab; enable_defer_to_tac;
-        unif_allow_ref_guards; erase_erasable_args; core_check;
-        missing_decl;_} -> solver
+        unif_allow_ref_guards; erase_erasable_args; core_check; missing_decl;
+        pending_lemmas;_} -> solver
 let (__proj__Mkenv__item__range : env -> FStar_Compiler_Range_Type.range) =
   fun projectee ->
     match projectee with
@@ -626,8 +713,8 @@ let (__proj__Mkenv__item__range : env -> FStar_Compiler_Range_Type.range) =
         fv_delta_depths; proof_ns; synth_hook; try_solve_implicits_hook;
         splice; mpreprocess; postprocess; identifier_info; tc_hooks; 
         dsenv; nbe; strict_args_tab; erasable_types_tab; enable_defer_to_tac;
-        unif_allow_ref_guards; erase_erasable_args; core_check;
-        missing_decl;_} -> range
+        unif_allow_ref_guards; erase_erasable_args; core_check; missing_decl;
+        pending_lemmas;_} -> range
 let (__proj__Mkenv__item__curmodule : env -> FStar_Ident.lident) =
   fun projectee ->
     match projectee with
@@ -641,8 +728,8 @@ let (__proj__Mkenv__item__curmodule : env -> FStar_Ident.lident) =
         fv_delta_depths; proof_ns; synth_hook; try_solve_implicits_hook;
         splice; mpreprocess; postprocess; identifier_info; tc_hooks; 
         dsenv; nbe; strict_args_tab; erasable_types_tab; enable_defer_to_tac;
-        unif_allow_ref_guards; erase_erasable_args; core_check;
-        missing_decl;_} -> curmodule
+        unif_allow_ref_guards; erase_erasable_args; core_check; missing_decl;
+        pending_lemmas;_} -> curmodule
 let (__proj__Mkenv__item__gamma :
   env -> FStar_Syntax_Syntax.binding Prims.list) =
   fun projectee ->
@@ -657,8 +744,8 @@ let (__proj__Mkenv__item__gamma :
         fv_delta_depths; proof_ns; synth_hook; try_solve_implicits_hook;
         splice; mpreprocess; postprocess; identifier_info; tc_hooks; 
         dsenv; nbe; strict_args_tab; erasable_types_tab; enable_defer_to_tac;
-        unif_allow_ref_guards; erase_erasable_args; core_check;
-        missing_decl;_} -> gamma
+        unif_allow_ref_guards; erase_erasable_args; core_check; missing_decl;
+        pending_lemmas;_} -> gamma
 let (__proj__Mkenv__item__gamma_sig : env -> sig_binding Prims.list) =
   fun projectee ->
     match projectee with
@@ -672,8 +759,8 @@ let (__proj__Mkenv__item__gamma_sig : env -> sig_binding Prims.list) =
         fv_delta_depths; proof_ns; synth_hook; try_solve_implicits_hook;
         splice; mpreprocess; postprocess; identifier_info; tc_hooks; 
         dsenv; nbe; strict_args_tab; erasable_types_tab; enable_defer_to_tac;
-        unif_allow_ref_guards; erase_erasable_args; core_check;
-        missing_decl;_} -> gamma_sig
+        unif_allow_ref_guards; erase_erasable_args; core_check; missing_decl;
+        pending_lemmas;_} -> gamma_sig
 let (__proj__Mkenv__item__gamma_cache :
   env -> cached_elt FStar_Compiler_Util.smap) =
   fun projectee ->
@@ -688,8 +775,8 @@ let (__proj__Mkenv__item__gamma_cache :
         fv_delta_depths; proof_ns; synth_hook; try_solve_implicits_hook;
         splice; mpreprocess; postprocess; identifier_info; tc_hooks; 
         dsenv; nbe; strict_args_tab; erasable_types_tab; enable_defer_to_tac;
-        unif_allow_ref_guards; erase_erasable_args; core_check;
-        missing_decl;_} -> gamma_cache
+        unif_allow_ref_guards; erase_erasable_args; core_check; missing_decl;
+        pending_lemmas;_} -> gamma_cache
 let (__proj__Mkenv__item__modules :
   env -> FStar_Syntax_Syntax.modul Prims.list) =
   fun projectee ->
@@ -704,8 +791,8 @@ let (__proj__Mkenv__item__modules :
         fv_delta_depths; proof_ns; synth_hook; try_solve_implicits_hook;
         splice; mpreprocess; postprocess; identifier_info; tc_hooks; 
         dsenv; nbe; strict_args_tab; erasable_types_tab; enable_defer_to_tac;
-        unif_allow_ref_guards; erase_erasable_args; core_check;
-        missing_decl;_} -> modules
+        unif_allow_ref_guards; erase_erasable_args; core_check; missing_decl;
+        pending_lemmas;_} -> modules
 let (__proj__Mkenv__item__expected_typ :
   env ->
     (FStar_Syntax_Syntax.typ * Prims.bool) FStar_Pervasives_Native.option)
@@ -722,8 +809,8 @@ let (__proj__Mkenv__item__expected_typ :
         fv_delta_depths; proof_ns; synth_hook; try_solve_implicits_hook;
         splice; mpreprocess; postprocess; identifier_info; tc_hooks; 
         dsenv; nbe; strict_args_tab; erasable_types_tab; enable_defer_to_tac;
-        unif_allow_ref_guards; erase_erasable_args; core_check;
-        missing_decl;_} -> expected_typ
+        unif_allow_ref_guards; erase_erasable_args; core_check; missing_decl;
+        pending_lemmas;_} -> expected_typ
 let (__proj__Mkenv__item__sigtab :
   env -> FStar_Syntax_Syntax.sigelt FStar_Compiler_Util.smap) =
   fun projectee ->
@@ -738,8 +825,8 @@ let (__proj__Mkenv__item__sigtab :
         fv_delta_depths; proof_ns; synth_hook; try_solve_implicits_hook;
         splice; mpreprocess; postprocess; identifier_info; tc_hooks; 
         dsenv; nbe; strict_args_tab; erasable_types_tab; enable_defer_to_tac;
-        unif_allow_ref_guards; erase_erasable_args; core_check;
-        missing_decl;_} -> sigtab
+        unif_allow_ref_guards; erase_erasable_args; core_check; missing_decl;
+        pending_lemmas;_} -> sigtab
 let (__proj__Mkenv__item__attrtab :
   env -> FStar_Syntax_Syntax.sigelt Prims.list FStar_Compiler_Util.smap) =
   fun projectee ->
@@ -754,8 +841,8 @@ let (__proj__Mkenv__item__attrtab :
         fv_delta_depths; proof_ns; synth_hook; try_solve_implicits_hook;
         splice; mpreprocess; postprocess; identifier_info; tc_hooks; 
         dsenv; nbe; strict_args_tab; erasable_types_tab; enable_defer_to_tac;
-        unif_allow_ref_guards; erase_erasable_args; core_check;
-        missing_decl;_} -> attrtab
+        unif_allow_ref_guards; erase_erasable_args; core_check; missing_decl;
+        pending_lemmas;_} -> attrtab
 let (__proj__Mkenv__item__instantiate_imp : env -> Prims.bool) =
   fun projectee ->
     match projectee with
@@ -769,8 +856,8 @@ let (__proj__Mkenv__item__instantiate_imp : env -> Prims.bool) =
         fv_delta_depths; proof_ns; synth_hook; try_solve_implicits_hook;
         splice; mpreprocess; postprocess; identifier_info; tc_hooks; 
         dsenv; nbe; strict_args_tab; erasable_types_tab; enable_defer_to_tac;
-        unif_allow_ref_guards; erase_erasable_args; core_check;
-        missing_decl;_} -> instantiate_imp
+        unif_allow_ref_guards; erase_erasable_args; core_check; missing_decl;
+        pending_lemmas;_} -> instantiate_imp
 let (__proj__Mkenv__item__effects : env -> effects) =
   fun projectee ->
     match projectee with
@@ -784,8 +871,8 @@ let (__proj__Mkenv__item__effects : env -> effects) =
         fv_delta_depths; proof_ns; synth_hook; try_solve_implicits_hook;
         splice; mpreprocess; postprocess; identifier_info; tc_hooks; 
         dsenv; nbe; strict_args_tab; erasable_types_tab; enable_defer_to_tac;
-        unif_allow_ref_guards; erase_erasable_args; core_check;
-        missing_decl;_} -> effects1
+        unif_allow_ref_guards; erase_erasable_args; core_check; missing_decl;
+        pending_lemmas;_} -> effects1
 let (__proj__Mkenv__item__generalize : env -> Prims.bool) =
   fun projectee ->
     match projectee with
@@ -799,8 +886,8 @@ let (__proj__Mkenv__item__generalize : env -> Prims.bool) =
         fv_delta_depths; proof_ns; synth_hook; try_solve_implicits_hook;
         splice; mpreprocess; postprocess; identifier_info; tc_hooks; 
         dsenv; nbe; strict_args_tab; erasable_types_tab; enable_defer_to_tac;
-        unif_allow_ref_guards; erase_erasable_args; core_check;
-        missing_decl;_} -> generalize
+        unif_allow_ref_guards; erase_erasable_args; core_check; missing_decl;
+        pending_lemmas;_} -> generalize
 let (__proj__Mkenv__item__letrecs :
   env ->
     (FStar_Syntax_Syntax.lbname * Prims.int * FStar_Syntax_Syntax.typ *
@@ -818,8 +905,8 @@ let (__proj__Mkenv__item__letrecs :
         fv_delta_depths; proof_ns; synth_hook; try_solve_implicits_hook;
         splice; mpreprocess; postprocess; identifier_info; tc_hooks; 
         dsenv; nbe; strict_args_tab; erasable_types_tab; enable_defer_to_tac;
-        unif_allow_ref_guards; erase_erasable_args; core_check;
-        missing_decl;_} -> letrecs
+        unif_allow_ref_guards; erase_erasable_args; core_check; missing_decl;
+        pending_lemmas;_} -> letrecs
 let (__proj__Mkenv__item__top_level : env -> Prims.bool) =
   fun projectee ->
     match projectee with
@@ -833,8 +920,8 @@ let (__proj__Mkenv__item__top_level : env -> Prims.bool) =
         fv_delta_depths; proof_ns; synth_hook; try_solve_implicits_hook;
         splice; mpreprocess; postprocess; identifier_info; tc_hooks; 
         dsenv; nbe; strict_args_tab; erasable_types_tab; enable_defer_to_tac;
-        unif_allow_ref_guards; erase_erasable_args; core_check;
-        missing_decl;_} -> top_level
+        unif_allow_ref_guards; erase_erasable_args; core_check; missing_decl;
+        pending_lemmas;_} -> top_level
 let (__proj__Mkenv__item__check_uvars : env -> Prims.bool) =
   fun projectee ->
     match projectee with
@@ -848,8 +935,8 @@ let (__proj__Mkenv__item__check_uvars : env -> Prims.bool) =
         fv_delta_depths; proof_ns; synth_hook; try_solve_implicits_hook;
         splice; mpreprocess; postprocess; identifier_info; tc_hooks; 
         dsenv; nbe; strict_args_tab; erasable_types_tab; enable_defer_to_tac;
-        unif_allow_ref_guards; erase_erasable_args; core_check;
-        missing_decl;_} -> check_uvars
+        unif_allow_ref_guards; erase_erasable_args; core_check; missing_decl;
+        pending_lemmas;_} -> check_uvars
 let (__proj__Mkenv__item__use_eq_strict : env -> Prims.bool) =
   fun projectee ->
     match projectee with
@@ -863,8 +950,8 @@ let (__proj__Mkenv__item__use_eq_strict : env -> Prims.bool) =
         fv_delta_depths; proof_ns; synth_hook; try_solve_implicits_hook;
         splice; mpreprocess; postprocess; identifier_info; tc_hooks; 
         dsenv; nbe; strict_args_tab; erasable_types_tab; enable_defer_to_tac;
-        unif_allow_ref_guards; erase_erasable_args; core_check;
-        missing_decl;_} -> use_eq_strict
+        unif_allow_ref_guards; erase_erasable_args; core_check; missing_decl;
+        pending_lemmas;_} -> use_eq_strict
 let (__proj__Mkenv__item__is_iface : env -> Prims.bool) =
   fun projectee ->
     match projectee with
@@ -878,8 +965,8 @@ let (__proj__Mkenv__item__is_iface : env -> Prims.bool) =
         fv_delta_depths; proof_ns; synth_hook; try_solve_implicits_hook;
         splice; mpreprocess; postprocess; identifier_info; tc_hooks; 
         dsenv; nbe; strict_args_tab; erasable_types_tab; enable_defer_to_tac;
-        unif_allow_ref_guards; erase_erasable_args; core_check;
-        missing_decl;_} -> is_iface
+        unif_allow_ref_guards; erase_erasable_args; core_check; missing_decl;
+        pending_lemmas;_} -> is_iface
 let (__proj__Mkenv__item__admit : env -> Prims.bool) =
   fun projectee ->
     match projectee with
@@ -893,8 +980,8 @@ let (__proj__Mkenv__item__admit : env -> Prims.bool) =
         fv_delta_depths; proof_ns; synth_hook; try_solve_implicits_hook;
         splice; mpreprocess; postprocess; identifier_info; tc_hooks; 
         dsenv; nbe; strict_args_tab; erasable_types_tab; enable_defer_to_tac;
-        unif_allow_ref_guards; erase_erasable_args; core_check;
-        missing_decl;_} -> admit
+        unif_allow_ref_guards; erase_erasable_args; core_check; missing_decl;
+        pending_lemmas;_} -> admit
 let (__proj__Mkenv__item__lax_universes : env -> Prims.bool) =
   fun projectee ->
     match projectee with
@@ -908,8 +995,8 @@ let (__proj__Mkenv__item__lax_universes : env -> Prims.bool) =
         fv_delta_depths; proof_ns; synth_hook; try_solve_implicits_hook;
         splice; mpreprocess; postprocess; identifier_info; tc_hooks; 
         dsenv; nbe; strict_args_tab; erasable_types_tab; enable_defer_to_tac;
-        unif_allow_ref_guards; erase_erasable_args; core_check;
-        missing_decl;_} -> lax_universes
+        unif_allow_ref_guards; erase_erasable_args; core_check; missing_decl;
+        pending_lemmas;_} -> lax_universes
 let (__proj__Mkenv__item__phase1 : env -> Prims.bool) =
   fun projectee ->
     match projectee with
@@ -923,8 +1010,8 @@ let (__proj__Mkenv__item__phase1 : env -> Prims.bool) =
         fv_delta_depths; proof_ns; synth_hook; try_solve_implicits_hook;
         splice; mpreprocess; postprocess; identifier_info; tc_hooks; 
         dsenv; nbe; strict_args_tab; erasable_types_tab; enable_defer_to_tac;
-        unif_allow_ref_guards; erase_erasable_args; core_check;
-        missing_decl;_} -> phase1
+        unif_allow_ref_guards; erase_erasable_args; core_check; missing_decl;
+        pending_lemmas;_} -> phase1
 let (__proj__Mkenv__item__failhard : env -> Prims.bool) =
   fun projectee ->
     match projectee with
@@ -938,8 +1025,8 @@ let (__proj__Mkenv__item__failhard : env -> Prims.bool) =
         fv_delta_depths; proof_ns; synth_hook; try_solve_implicits_hook;
         splice; mpreprocess; postprocess; identifier_info; tc_hooks; 
         dsenv; nbe; strict_args_tab; erasable_types_tab; enable_defer_to_tac;
-        unif_allow_ref_guards; erase_erasable_args; core_check;
-        missing_decl;_} -> failhard
+        unif_allow_ref_guards; erase_erasable_args; core_check; missing_decl;
+        pending_lemmas;_} -> failhard
 let (__proj__Mkenv__item__flychecking : env -> Prims.bool) =
   fun projectee ->
     match projectee with
@@ -953,8 +1040,8 @@ let (__proj__Mkenv__item__flychecking : env -> Prims.bool) =
         fv_delta_depths; proof_ns; synth_hook; try_solve_implicits_hook;
         splice; mpreprocess; postprocess; identifier_info; tc_hooks; 
         dsenv; nbe; strict_args_tab; erasable_types_tab; enable_defer_to_tac;
-        unif_allow_ref_guards; erase_erasable_args; core_check;
-        missing_decl;_} -> flychecking
+        unif_allow_ref_guards; erase_erasable_args; core_check; missing_decl;
+        pending_lemmas;_} -> flychecking
 let (__proj__Mkenv__item__uvar_subtyping : env -> Prims.bool) =
   fun projectee ->
     match projectee with
@@ -968,8 +1055,8 @@ let (__proj__Mkenv__item__uvar_subtyping : env -> Prims.bool) =
         fv_delta_depths; proof_ns; synth_hook; try_solve_implicits_hook;
         splice; mpreprocess; postprocess; identifier_info; tc_hooks; 
         dsenv; nbe; strict_args_tab; erasable_types_tab; enable_defer_to_tac;
-        unif_allow_ref_guards; erase_erasable_args; core_check;
-        missing_decl;_} -> uvar_subtyping
+        unif_allow_ref_guards; erase_erasable_args; core_check; missing_decl;
+        pending_lemmas;_} -> uvar_subtyping
 let (__proj__Mkenv__item__intactics : env -> Prims.bool) =
   fun projectee ->
     match projectee with
@@ -983,8 +1070,8 @@ let (__proj__Mkenv__item__intactics : env -> Prims.bool) =
         fv_delta_depths; proof_ns; synth_hook; try_solve_implicits_hook;
         splice; mpreprocess; postprocess; identifier_info; tc_hooks; 
         dsenv; nbe; strict_args_tab; erasable_types_tab; enable_defer_to_tac;
-        unif_allow_ref_guards; erase_erasable_args; core_check;
-        missing_decl;_} -> intactics
+        unif_allow_ref_guards; erase_erasable_args; core_check; missing_decl;
+        pending_lemmas;_} -> intactics
 let (__proj__Mkenv__item__nocoerce : env -> Prims.bool) =
   fun projectee ->
     match projectee with
@@ -998,8 +1085,8 @@ let (__proj__Mkenv__item__nocoerce : env -> Prims.bool) =
         fv_delta_depths; proof_ns; synth_hook; try_solve_implicits_hook;
         splice; mpreprocess; postprocess; identifier_info; tc_hooks; 
         dsenv; nbe; strict_args_tab; erasable_types_tab; enable_defer_to_tac;
-        unif_allow_ref_guards; erase_erasable_args; core_check;
-        missing_decl;_} -> nocoerce
+        unif_allow_ref_guards; erase_erasable_args; core_check; missing_decl;
+        pending_lemmas;_} -> nocoerce
 let (__proj__Mkenv__item__tc_term :
   env ->
     env ->
@@ -1019,8 +1106,8 @@ let (__proj__Mkenv__item__tc_term :
         fv_delta_depths; proof_ns; synth_hook; try_solve_implicits_hook;
         splice; mpreprocess; postprocess; identifier_info; tc_hooks; 
         dsenv; nbe; strict_args_tab; erasable_types_tab; enable_defer_to_tac;
-        unif_allow_ref_guards; erase_erasable_args; core_check;
-        missing_decl;_} -> tc_term
+        unif_allow_ref_guards; erase_erasable_args; core_check; missing_decl;
+        pending_lemmas;_} -> tc_term
 let (__proj__Mkenv__item__typeof_tot_or_gtot_term :
   env ->
     env ->
@@ -1041,8 +1128,8 @@ let (__proj__Mkenv__item__typeof_tot_or_gtot_term :
         fv_delta_depths; proof_ns; synth_hook; try_solve_implicits_hook;
         splice; mpreprocess; postprocess; identifier_info; tc_hooks; 
         dsenv; nbe; strict_args_tab; erasable_types_tab; enable_defer_to_tac;
-        unif_allow_ref_guards; erase_erasable_args; core_check;
-        missing_decl;_} -> typeof_tot_or_gtot_term
+        unif_allow_ref_guards; erase_erasable_args; core_check; missing_decl;
+        pending_lemmas;_} -> typeof_tot_or_gtot_term
 let (__proj__Mkenv__item__universe_of :
   env -> env -> FStar_Syntax_Syntax.term -> FStar_Syntax_Syntax.universe) =
   fun projectee ->
@@ -1057,8 +1144,8 @@ let (__proj__Mkenv__item__universe_of :
         fv_delta_depths; proof_ns; synth_hook; try_solve_implicits_hook;
         splice; mpreprocess; postprocess; identifier_info; tc_hooks; 
         dsenv; nbe; strict_args_tab; erasable_types_tab; enable_defer_to_tac;
-        unif_allow_ref_guards; erase_erasable_args; core_check;
-        missing_decl;_} -> universe_of
+        unif_allow_ref_guards; erase_erasable_args; core_check; missing_decl;
+        pending_lemmas;_} -> universe_of
 let (__proj__Mkenv__item__typeof_well_typed_tot_or_gtot_term :
   env ->
     env ->
@@ -1078,8 +1165,8 @@ let (__proj__Mkenv__item__typeof_well_typed_tot_or_gtot_term :
         fv_delta_depths; proof_ns; synth_hook; try_solve_implicits_hook;
         splice; mpreprocess; postprocess; identifier_info; tc_hooks; 
         dsenv; nbe; strict_args_tab; erasable_types_tab; enable_defer_to_tac;
-        unif_allow_ref_guards; erase_erasable_args; core_check;
-        missing_decl;_} -> typeof_well_typed_tot_or_gtot_term
+        unif_allow_ref_guards; erase_erasable_args; core_check; missing_decl;
+        pending_lemmas;_} -> typeof_well_typed_tot_or_gtot_term
 let (__proj__Mkenv__item__teq_nosmt_force :
   env ->
     env -> FStar_Syntax_Syntax.term -> FStar_Syntax_Syntax.term -> Prims.bool)
@@ -1096,8 +1183,8 @@ let (__proj__Mkenv__item__teq_nosmt_force :
         fv_delta_depths; proof_ns; synth_hook; try_solve_implicits_hook;
         splice; mpreprocess; postprocess; identifier_info; tc_hooks; 
         dsenv; nbe; strict_args_tab; erasable_types_tab; enable_defer_to_tac;
-        unif_allow_ref_guards; erase_erasable_args; core_check;
-        missing_decl;_} -> teq_nosmt_force
+        unif_allow_ref_guards; erase_erasable_args; core_check; missing_decl;
+        pending_lemmas;_} -> teq_nosmt_force
 let (__proj__Mkenv__item__subtype_nosmt_force :
   env ->
     env -> FStar_Syntax_Syntax.term -> FStar_Syntax_Syntax.term -> Prims.bool)
@@ -1114,8 +1201,8 @@ let (__proj__Mkenv__item__subtype_nosmt_force :
         fv_delta_depths; proof_ns; synth_hook; try_solve_implicits_hook;
         splice; mpreprocess; postprocess; identifier_info; tc_hooks; 
         dsenv; nbe; strict_args_tab; erasable_types_tab; enable_defer_to_tac;
-        unif_allow_ref_guards; erase_erasable_args; core_check;
-        missing_decl;_} -> subtype_nosmt_force
+        unif_allow_ref_guards; erase_erasable_args; core_check; missing_decl;
+        pending_lemmas;_} -> subtype_nosmt_force
 let (__proj__Mkenv__item__qtbl_name_and_index :
   env ->
     ((FStar_Ident.lident * FStar_Syntax_Syntax.typ * Prims.int)
@@ -1133,8 +1220,8 @@ let (__proj__Mkenv__item__qtbl_name_and_index :
         fv_delta_depths; proof_ns; synth_hook; try_solve_implicits_hook;
         splice; mpreprocess; postprocess; identifier_info; tc_hooks; 
         dsenv; nbe; strict_args_tab; erasable_types_tab; enable_defer_to_tac;
-        unif_allow_ref_guards; erase_erasable_args; core_check;
-        missing_decl;_} -> qtbl_name_and_index
+        unif_allow_ref_guards; erase_erasable_args; core_check; missing_decl;
+        pending_lemmas;_} -> qtbl_name_and_index
 let (__proj__Mkenv__item__normalized_eff_names :
   env -> FStar_Ident.lident FStar_Compiler_Util.smap) =
   fun projectee ->
@@ -1149,8 +1236,8 @@ let (__proj__Mkenv__item__normalized_eff_names :
         fv_delta_depths; proof_ns; synth_hook; try_solve_implicits_hook;
         splice; mpreprocess; postprocess; identifier_info; tc_hooks; 
         dsenv; nbe; strict_args_tab; erasable_types_tab; enable_defer_to_tac;
-        unif_allow_ref_guards; erase_erasable_args; core_check;
-        missing_decl;_} -> normalized_eff_names
+        unif_allow_ref_guards; erase_erasable_args; core_check; missing_decl;
+        pending_lemmas;_} -> normalized_eff_names
 let (__proj__Mkenv__item__fv_delta_depths :
   env -> FStar_Syntax_Syntax.delta_depth FStar_Compiler_Util.smap) =
   fun projectee ->
@@ -1165,8 +1252,8 @@ let (__proj__Mkenv__item__fv_delta_depths :
         fv_delta_depths; proof_ns; synth_hook; try_solve_implicits_hook;
         splice; mpreprocess; postprocess; identifier_info; tc_hooks; 
         dsenv; nbe; strict_args_tab; erasable_types_tab; enable_defer_to_tac;
-        unif_allow_ref_guards; erase_erasable_args; core_check;
-        missing_decl;_} -> fv_delta_depths
+        unif_allow_ref_guards; erase_erasable_args; core_check; missing_decl;
+        pending_lemmas;_} -> fv_delta_depths
 let (__proj__Mkenv__item__proof_ns : env -> proof_namespace) =
   fun projectee ->
     match projectee with
@@ -1180,8 +1267,8 @@ let (__proj__Mkenv__item__proof_ns : env -> proof_namespace) =
         fv_delta_depths; proof_ns; synth_hook; try_solve_implicits_hook;
         splice; mpreprocess; postprocess; identifier_info; tc_hooks; 
         dsenv; nbe; strict_args_tab; erasable_types_tab; enable_defer_to_tac;
-        unif_allow_ref_guards; erase_erasable_args; core_check;
-        missing_decl;_} -> proof_ns
+        unif_allow_ref_guards; erase_erasable_args; core_check; missing_decl;
+        pending_lemmas;_} -> proof_ns
 let (__proj__Mkenv__item__synth_hook :
   env ->
     env ->
@@ -1200,8 +1287,8 @@ let (__proj__Mkenv__item__synth_hook :
         fv_delta_depths; proof_ns; synth_hook; try_solve_implicits_hook;
         splice; mpreprocess; postprocess; identifier_info; tc_hooks; 
         dsenv; nbe; strict_args_tab; erasable_types_tab; enable_defer_to_tac;
-        unif_allow_ref_guards; erase_erasable_args; core_check;
-        missing_decl;_} -> synth_hook
+        unif_allow_ref_guards; erase_erasable_args; core_check; missing_decl;
+        pending_lemmas;_} -> synth_hook
 let (__proj__Mkenv__item__try_solve_implicits_hook :
   env ->
     env ->
@@ -1219,8 +1306,8 @@ let (__proj__Mkenv__item__try_solve_implicits_hook :
         fv_delta_depths; proof_ns; synth_hook; try_solve_implicits_hook;
         splice; mpreprocess; postprocess; identifier_info; tc_hooks; 
         dsenv; nbe; strict_args_tab; erasable_types_tab; enable_defer_to_tac;
-        unif_allow_ref_guards; erase_erasable_args; core_check;
-        missing_decl;_} -> try_solve_implicits_hook
+        unif_allow_ref_guards; erase_erasable_args; core_check; missing_decl;
+        pending_lemmas;_} -> try_solve_implicits_hook
 let (__proj__Mkenv__item__splice :
   env ->
     env ->
@@ -1242,8 +1329,8 @@ let (__proj__Mkenv__item__splice :
         fv_delta_depths; proof_ns; synth_hook; try_solve_implicits_hook;
         splice; mpreprocess; postprocess; identifier_info; tc_hooks; 
         dsenv; nbe; strict_args_tab; erasable_types_tab; enable_defer_to_tac;
-        unif_allow_ref_guards; erase_erasable_args; core_check;
-        missing_decl;_} -> splice
+        unif_allow_ref_guards; erase_erasable_args; core_check; missing_decl;
+        pending_lemmas;_} -> splice
 let (__proj__Mkenv__item__mpreprocess :
   env ->
     env ->
@@ -1262,8 +1349,8 @@ let (__proj__Mkenv__item__mpreprocess :
         fv_delta_depths; proof_ns; synth_hook; try_solve_implicits_hook;
         splice; mpreprocess; postprocess; identifier_info; tc_hooks; 
         dsenv; nbe; strict_args_tab; erasable_types_tab; enable_defer_to_tac;
-        unif_allow_ref_guards; erase_erasable_args; core_check;
-        missing_decl;_} -> mpreprocess
+        unif_allow_ref_guards; erase_erasable_args; core_check; missing_decl;
+        pending_lemmas;_} -> mpreprocess
 let (__proj__Mkenv__item__postprocess :
   env ->
     env ->
@@ -1283,8 +1370,8 @@ let (__proj__Mkenv__item__postprocess :
         fv_delta_depths; proof_ns; synth_hook; try_solve_implicits_hook;
         splice; mpreprocess; postprocess; identifier_info; tc_hooks; 
         dsenv; nbe; strict_args_tab; erasable_types_tab; enable_defer_to_tac;
-        unif_allow_ref_guards; erase_erasable_args; core_check;
-        missing_decl;_} -> postprocess
+        unif_allow_ref_guards; erase_erasable_args; core_check; missing_decl;
+        pending_lemmas;_} -> postprocess
 let (__proj__Mkenv__item__identifier_info :
   env -> FStar_TypeChecker_Common.id_info_table FStar_Compiler_Effect.ref) =
   fun projectee ->
@@ -1299,8 +1386,8 @@ let (__proj__Mkenv__item__identifier_info :
         fv_delta_depths; proof_ns; synth_hook; try_solve_implicits_hook;
         splice; mpreprocess; postprocess; identifier_info; tc_hooks; 
         dsenv; nbe; strict_args_tab; erasable_types_tab; enable_defer_to_tac;
-        unif_allow_ref_guards; erase_erasable_args; core_check;
-        missing_decl;_} -> identifier_info
+        unif_allow_ref_guards; erase_erasable_args; core_check; missing_decl;
+        pending_lemmas;_} -> identifier_info
 let (__proj__Mkenv__item__tc_hooks : env -> tcenv_hooks) =
   fun projectee ->
     match projectee with
@@ -1314,8 +1401,8 @@ let (__proj__Mkenv__item__tc_hooks : env -> tcenv_hooks) =
         fv_delta_depths; proof_ns; synth_hook; try_solve_implicits_hook;
         splice; mpreprocess; postprocess; identifier_info; tc_hooks; 
         dsenv; nbe; strict_args_tab; erasable_types_tab; enable_defer_to_tac;
-        unif_allow_ref_guards; erase_erasable_args; core_check;
-        missing_decl;_} -> tc_hooks
+        unif_allow_ref_guards; erase_erasable_args; core_check; missing_decl;
+        pending_lemmas;_} -> tc_hooks
 let (__proj__Mkenv__item__dsenv : env -> FStar_Syntax_DsEnv.env) =
   fun projectee ->
     match projectee with
@@ -1329,8 +1416,8 @@ let (__proj__Mkenv__item__dsenv : env -> FStar_Syntax_DsEnv.env) =
         fv_delta_depths; proof_ns; synth_hook; try_solve_implicits_hook;
         splice; mpreprocess; postprocess; identifier_info; tc_hooks; 
         dsenv; nbe; strict_args_tab; erasable_types_tab; enable_defer_to_tac;
-        unif_allow_ref_guards; erase_erasable_args; core_check;
-        missing_decl;_} -> dsenv
+        unif_allow_ref_guards; erase_erasable_args; core_check; missing_decl;
+        pending_lemmas;_} -> dsenv
 let (__proj__Mkenv__item__nbe :
   env ->
     step Prims.list ->
@@ -1348,8 +1435,8 @@ let (__proj__Mkenv__item__nbe :
         fv_delta_depths; proof_ns; synth_hook; try_solve_implicits_hook;
         splice; mpreprocess; postprocess; identifier_info; tc_hooks; 
         dsenv; nbe; strict_args_tab; erasable_types_tab; enable_defer_to_tac;
-        unif_allow_ref_guards; erase_erasable_args; core_check;
-        missing_decl;_} -> nbe
+        unif_allow_ref_guards; erase_erasable_args; core_check; missing_decl;
+        pending_lemmas;_} -> nbe
 let (__proj__Mkenv__item__strict_args_tab :
   env ->
     Prims.int Prims.list FStar_Pervasives_Native.option
@@ -1367,8 +1454,8 @@ let (__proj__Mkenv__item__strict_args_tab :
         fv_delta_depths; proof_ns; synth_hook; try_solve_implicits_hook;
         splice; mpreprocess; postprocess; identifier_info; tc_hooks; 
         dsenv; nbe; strict_args_tab; erasable_types_tab; enable_defer_to_tac;
-        unif_allow_ref_guards; erase_erasable_args; core_check;
-        missing_decl;_} -> strict_args_tab
+        unif_allow_ref_guards; erase_erasable_args; core_check; missing_decl;
+        pending_lemmas;_} -> strict_args_tab
 let (__proj__Mkenv__item__erasable_types_tab :
   env -> Prims.bool FStar_Compiler_Util.smap) =
   fun projectee ->
@@ -1383,8 +1470,8 @@ let (__proj__Mkenv__item__erasable_types_tab :
         fv_delta_depths; proof_ns; synth_hook; try_solve_implicits_hook;
         splice; mpreprocess; postprocess; identifier_info; tc_hooks; 
         dsenv; nbe; strict_args_tab; erasable_types_tab; enable_defer_to_tac;
-        unif_allow_ref_guards; erase_erasable_args; core_check;
-        missing_decl;_} -> erasable_types_tab
+        unif_allow_ref_guards; erase_erasable_args; core_check; missing_decl;
+        pending_lemmas;_} -> erasable_types_tab
 let (__proj__Mkenv__item__enable_defer_to_tac : env -> Prims.bool) =
   fun projectee ->
     match projectee with
@@ -1398,8 +1485,8 @@ let (__proj__Mkenv__item__enable_defer_to_tac : env -> Prims.bool) =
         fv_delta_depths; proof_ns; synth_hook; try_solve_implicits_hook;
         splice; mpreprocess; postprocess; identifier_info; tc_hooks; 
         dsenv; nbe; strict_args_tab; erasable_types_tab; enable_defer_to_tac;
-        unif_allow_ref_guards; erase_erasable_args; core_check;
-        missing_decl;_} -> enable_defer_to_tac
+        unif_allow_ref_guards; erase_erasable_args; core_check; missing_decl;
+        pending_lemmas;_} -> enable_defer_to_tac
 let (__proj__Mkenv__item__unif_allow_ref_guards : env -> Prims.bool) =
   fun projectee ->
     match projectee with
@@ -1413,8 +1500,8 @@ let (__proj__Mkenv__item__unif_allow_ref_guards : env -> Prims.bool) =
         fv_delta_depths; proof_ns; synth_hook; try_solve_implicits_hook;
         splice; mpreprocess; postprocess; identifier_info; tc_hooks; 
         dsenv; nbe; strict_args_tab; erasable_types_tab; enable_defer_to_tac;
-        unif_allow_ref_guards; erase_erasable_args; core_check;
-        missing_decl;_} -> unif_allow_ref_guards
+        unif_allow_ref_guards; erase_erasable_args; core_check; missing_decl;
+        pending_lemmas;_} -> unif_allow_ref_guards
 let (__proj__Mkenv__item__erase_erasable_args : env -> Prims.bool) =
   fun projectee ->
     match projectee with
@@ -1428,8 +1515,8 @@ let (__proj__Mkenv__item__erase_erasable_args : env -> Prims.bool) =
         fv_delta_depths; proof_ns; synth_hook; try_solve_implicits_hook;
         splice; mpreprocess; postprocess; identifier_info; tc_hooks; 
         dsenv; nbe; strict_args_tab; erasable_types_tab; enable_defer_to_tac;
-        unif_allow_ref_guards; erase_erasable_args; core_check;
-        missing_decl;_} -> erase_erasable_args
+        unif_allow_ref_guards; erase_erasable_args; core_check; missing_decl;
+        pending_lemmas;_} -> erase_erasable_args
 let (__proj__Mkenv__item__core_check :
   env ->
     env ->
@@ -1451,8 +1538,8 @@ let (__proj__Mkenv__item__core_check :
         fv_delta_depths; proof_ns; synth_hook; try_solve_implicits_hook;
         splice; mpreprocess; postprocess; identifier_info; tc_hooks; 
         dsenv; nbe; strict_args_tab; erasable_types_tab; enable_defer_to_tac;
-        unif_allow_ref_guards; erase_erasable_args; core_check;
-        missing_decl;_} -> core_check
+        unif_allow_ref_guards; erase_erasable_args; core_check; missing_decl;
+        pending_lemmas;_} -> core_check
 let (__proj__Mkenv__item__missing_decl :
   env -> FStar_Ident.lident FStar_Compiler_RBSet.t) =
   fun projectee ->
@@ -1467,8 +1554,23 @@ let (__proj__Mkenv__item__missing_decl :
         fv_delta_depths; proof_ns; synth_hook; try_solve_implicits_hook;
         splice; mpreprocess; postprocess; identifier_info; tc_hooks; 
         dsenv; nbe; strict_args_tab; erasable_types_tab; enable_defer_to_tac;
-        unif_allow_ref_guards; erase_erasable_args; core_check;
-        missing_decl;_} -> missing_decl
+        unif_allow_ref_guards; erase_erasable_args; core_check; missing_decl;
+        pending_lemmas;_} -> missing_decl
+let (__proj__Mkenv__item__pending_lemmas : env -> pending_lemma_patterns) =
+  fun projectee ->
+    match projectee with
+    | { solver; range; curmodule; gamma; gamma_sig; gamma_cache; modules;
+        expected_typ; sigtab; attrtab; instantiate_imp; effects = effects1;
+        generalize; letrecs; top_level; check_uvars; use_eq_strict; is_iface;
+        admit; lax_universes; phase1; failhard; flychecking; uvar_subtyping;
+        intactics; nocoerce; tc_term; typeof_tot_or_gtot_term; universe_of;
+        typeof_well_typed_tot_or_gtot_term; teq_nosmt_force;
+        subtype_nosmt_force; qtbl_name_and_index; normalized_eff_names;
+        fv_delta_depths; proof_ns; synth_hook; try_solve_implicits_hook;
+        splice; mpreprocess; postprocess; identifier_info; tc_hooks; 
+        dsenv; nbe; strict_args_tab; erasable_types_tab; enable_defer_to_tac;
+        unif_allow_ref_guards; erase_erasable_args; core_check; missing_decl;
+        pending_lemmas;_} -> pending_lemmas
 let (__proj__Mksolver_t__item__init : solver_t -> env -> unit) =
   fun projectee ->
     match projectee with
@@ -1701,7 +1803,8 @@ let (rename_env : FStar_Syntax_Syntax.subst_t -> env -> env) =
         unif_allow_ref_guards = (env1.unif_allow_ref_guards);
         erase_erasable_args = (env1.erase_erasable_args);
         core_check = (env1.core_check);
-        missing_decl = (env1.missing_decl)
+        missing_decl = (env1.missing_decl);
+        pending_lemmas = (env1.pending_lemmas)
       }
 let (default_tc_hooks : tcenv_hooks) =
   { tc_push_in_gamma_hook = (fun uu___ -> fun uu___1 -> ()) }
@@ -1762,7 +1865,8 @@ let (set_tc_hooks : env -> tcenv_hooks -> env) =
         unif_allow_ref_guards = (env1.unif_allow_ref_guards);
         erase_erasable_args = (env1.erase_erasable_args);
         core_check = (env1.core_check);
-        missing_decl = (env1.missing_decl)
+        missing_decl = (env1.missing_decl);
+        pending_lemmas = (env1.pending_lemmas)
       }
 let (set_dep_graph : env -> FStar_Parser_Dep.deps -> env) =
   fun e ->
@@ -1821,7 +1925,8 @@ let (set_dep_graph : env -> FStar_Parser_Dep.deps -> env) =
         unif_allow_ref_guards = (e.unif_allow_ref_guards);
         erase_erasable_args = (e.erase_erasable_args);
         core_check = (e.core_check);
-        missing_decl = (e.missing_decl)
+        missing_decl = (e.missing_decl);
+        pending_lemmas = (e.pending_lemmas)
       }
 let (dep_graph : env -> FStar_Parser_Dep.deps) =
   fun e -> FStar_Syntax_DsEnv.dep_graph e.dsenv
@@ -1887,7 +1992,8 @@ let (record_val_for : env -> FStar_Ident.lident -> env) =
         unif_allow_ref_guards = (e.unif_allow_ref_guards);
         erase_erasable_args = (e.erase_erasable_args);
         core_check = (e.core_check);
-        missing_decl = uu___
+        missing_decl = uu___;
+        pending_lemmas = (e.pending_lemmas)
       }
 let (record_definition_for : env -> FStar_Ident.lident -> env) =
   fun e ->
@@ -1951,7 +2057,8 @@ let (record_definition_for : env -> FStar_Ident.lident -> env) =
         unif_allow_ref_guards = (e.unif_allow_ref_guards);
         erase_erasable_args = (e.erase_erasable_args);
         core_check = (e.core_check);
-        missing_decl = uu___
+        missing_decl = uu___;
+        pending_lemmas = (e.pending_lemmas)
       }
 let (missing_definition_list : env -> FStar_Ident.lident Prims.list) =
   fun e ->
@@ -1959,17 +2066,6 @@ let (missing_definition_list : env -> FStar_Ident.lident Prims.list) =
       (Obj.magic
          (FStar_Compiler_RBSet.setlike_rbset FStar_Syntax_Syntax.ord_fv))
       (Obj.magic e.missing_decl)
-type implicit = FStar_TypeChecker_Common.implicit
-type implicits = FStar_TypeChecker_Common.implicits
-type guard_t = FStar_TypeChecker_Common.guard_t
-type tcenv_depth_t = (Prims.int * Prims.int * solver_depth_t * Prims.int)
-type qninfo =
-  (((FStar_Syntax_Syntax.universes * FStar_Syntax_Syntax.typ),
-    (FStar_Syntax_Syntax.sigelt * FStar_Syntax_Syntax.universes
-      FStar_Pervasives_Native.option))
-    FStar_Pervasives.either * FStar_Compiler_Range_Type.range)
-    FStar_Pervasives_Native.option
-type env_t = env
 type sigtable = FStar_Syntax_Syntax.sigelt FStar_Compiler_Util.smap
 let (should_verify : env -> Prims.bool) =
   fun env1 ->
@@ -2001,12 +2097,13 @@ let (initial_env :
     (env ->
        FStar_Syntax_Syntax.term ->
          (FStar_Syntax_Syntax.term * FStar_TypeChecker_Common.lcomp *
-           guard_t))
+           FStar_TypeChecker_Common.guard_t))
       ->
       (env ->
          FStar_Syntax_Syntax.term ->
            must_tot ->
-             (FStar_Syntax_Syntax.term * FStar_Syntax_Syntax.typ * guard_t))
+             (FStar_Syntax_Syntax.term * FStar_Syntax_Syntax.typ *
+               FStar_TypeChecker_Common.guard_t))
         ->
         (env ->
            FStar_Syntax_Syntax.term ->
@@ -2171,7 +2268,8 @@ let (initial_env :
                           unif_allow_ref_guards = false;
                           erase_erasable_args = false;
                           core_check;
-                          missing_decl = uu___11
+                          missing_decl = uu___11;
+                          pending_lemmas = empty_pending_lemma_patterns
                         }
 let (dsenv : env -> FStar_Syntax_DsEnv.env) = fun env1 -> env1.dsenv
 let (sigtab : env -> FStar_Syntax_Syntax.sigelt FStar_Compiler_Util.smap) =
@@ -2181,6 +2279,125 @@ let (attrtab :
   fun env1 -> env1.attrtab
 let (gamma_cache : env -> cached_elt FStar_Compiler_Util.smap) =
   fun env1 -> env1.gamma_cache
+let (maybe_add_pending_lemma :
+  env -> FStar_Ident.lident -> FStar_Syntax_Syntax.typ -> env) =
+  fun e ->
+    fun lem ->
+      fun t ->
+        let uu___ =
+          let uu___1 = FStar_Syntax_Util.is_smt_lemma t in
+          Prims.op_Negation uu___1 in
+        if uu___
+        then e
+        else
+          (let triggers = FStar_Syntax_Util.triggers_of_smt_lemma t in
+           let uu___2 = e.pending_lemmas in
+           match uu___2 with
+           | { pending_lemma_triggers; lidents_to_pending_lemmas;_} ->
+               let pending_lemma_triggers1 =
+                 let uu___3 = FStar_Ident.string_of_lid lem in
+                 FStar_Compiler_Util.psmap_add pending_lemma_triggers uu___3
+                   triggers in
+               let lidents_to_pending_lemmas1 =
+                 FStar_Compiler_List.fold_left
+                   (fun acc ->
+                      fun disjunct ->
+                        FStar_Compiler_List.fold_left
+                          (fun acc1 ->
+                             fun conjunct ->
+                               FStar_Compiler_List.fold_left
+                                 (fun acc2 ->
+                                    fun lident ->
+                                      let uu___3 =
+                                        let uu___4 =
+                                          FStar_Ident.string_of_lid lident in
+                                        FStar_Compiler_Util.psmap_try_find
+                                          lidents_to_pending_lemmas uu___4 in
+                                      match uu___3 with
+                                      | FStar_Pervasives_Native.None ->
+                                          let uu___4 =
+                                            FStar_Ident.string_of_lid lident in
+                                          FStar_Compiler_Util.psmap_add acc2
+                                            uu___4 [lem]
+                                      | FStar_Pervasives_Native.Some lems ->
+                                          let uu___4 =
+                                            FStar_Ident.string_of_lid lident in
+                                          FStar_Compiler_Util.psmap_add acc2
+                                            uu___4 (lem :: lems)) acc1
+                                 conjunct) acc disjunct)
+                   lidents_to_pending_lemmas triggers in
+               let p =
+                 {
+                   pending_lemma_triggers = pending_lemma_triggers1;
+                   lidents_to_pending_lemmas = lidents_to_pending_lemmas1
+                 } in
+               {
+                 solver = (e.solver);
+                 range = (e.range);
+                 curmodule = (e.curmodule);
+                 gamma = (e.gamma);
+                 gamma_sig = (e.gamma_sig);
+                 gamma_cache = (e.gamma_cache);
+                 modules = (e.modules);
+                 expected_typ = (e.expected_typ);
+                 sigtab = (e.sigtab);
+                 attrtab = (e.attrtab);
+                 instantiate_imp = (e.instantiate_imp);
+                 effects = (e.effects);
+                 generalize = (e.generalize);
+                 letrecs = (e.letrecs);
+                 top_level = (e.top_level);
+                 check_uvars = (e.check_uvars);
+                 use_eq_strict = (e.use_eq_strict);
+                 is_iface = (e.is_iface);
+                 admit = (e.admit);
+                 lax_universes = (e.lax_universes);
+                 phase1 = (e.phase1);
+                 failhard = (e.failhard);
+                 flychecking = (e.flychecking);
+                 uvar_subtyping = (e.uvar_subtyping);
+                 intactics = (e.intactics);
+                 nocoerce = (e.nocoerce);
+                 tc_term = (e.tc_term);
+                 typeof_tot_or_gtot_term = (e.typeof_tot_or_gtot_term);
+                 universe_of = (e.universe_of);
+                 typeof_well_typed_tot_or_gtot_term =
+                   (e.typeof_well_typed_tot_or_gtot_term);
+                 teq_nosmt_force = (e.teq_nosmt_force);
+                 subtype_nosmt_force = (e.subtype_nosmt_force);
+                 qtbl_name_and_index = (e.qtbl_name_and_index);
+                 normalized_eff_names = (e.normalized_eff_names);
+                 fv_delta_depths = (e.fv_delta_depths);
+                 proof_ns = (e.proof_ns);
+                 synth_hook = (e.synth_hook);
+                 try_solve_implicits_hook = (e.try_solve_implicits_hook);
+                 splice = (e.splice);
+                 mpreprocess = (e.mpreprocess);
+                 postprocess = (e.postprocess);
+                 identifier_info = (e.identifier_info);
+                 tc_hooks = (e.tc_hooks);
+                 dsenv = (e.dsenv);
+                 nbe = (e.nbe);
+                 strict_args_tab = (e.strict_args_tab);
+                 erasable_types_tab = (e.erasable_types_tab);
+                 enable_defer_to_tac = (e.enable_defer_to_tac);
+                 unif_allow_ref_guards = (e.unif_allow_ref_guards);
+                 erase_erasable_args = (e.erase_erasable_args);
+                 core_check = (e.core_check);
+                 missing_decl = (e.missing_decl);
+                 pending_lemmas = p
+               })
+type implicit = FStar_TypeChecker_Common.implicit
+type implicits = FStar_TypeChecker_Common.implicits
+type guard_t = FStar_TypeChecker_Common.guard_t
+type tcenv_depth_t = (Prims.int * Prims.int * solver_depth_t * Prims.int)
+type qninfo =
+  (((FStar_Syntax_Syntax.universes * FStar_Syntax_Syntax.typ),
+    (FStar_Syntax_Syntax.sigelt * FStar_Syntax_Syntax.universes
+      FStar_Pervasives_Native.option))
+    FStar_Pervasives.either * FStar_Compiler_Range_Type.range)
+    FStar_Pervasives_Native.option
+type env_t = env
 let (query_indices :
   (FStar_Ident.lident * Prims.int) Prims.list Prims.list
     FStar_Compiler_Effect.ref)
@@ -2299,7 +2516,8 @@ let (push_stack : env -> env) =
        unif_allow_ref_guards = (env1.unif_allow_ref_guards);
        erase_erasable_args = (env1.erase_erasable_args);
        core_check = (env1.core_check);
-       missing_decl = (env1.missing_decl)
+       missing_decl = (env1.missing_decl);
+       pending_lemmas = (env1.pending_lemmas)
      })
 let (pop_stack : unit -> env) =
   fun uu___ ->
@@ -2392,7 +2610,8 @@ let (snapshot : env -> Prims.string -> (tcenv_depth_t * env)) =
                                   erase_erasable_args =
                                     (env2.erase_erasable_args);
                                   core_check = (env2.core_check);
-                                  missing_decl = (env2.missing_decl)
+                                  missing_decl = (env2.missing_decl);
+                                  pending_lemmas = (env2.pending_lemmas)
                                 })))))
 let (rollback :
   solver_t ->
@@ -2511,7 +2730,8 @@ let (incr_query_index : env -> env) =
                 unif_allow_ref_guards = (env1.unif_allow_ref_guards);
                 erase_erasable_args = (env1.erase_erasable_args);
                 core_check = (env1.core_check);
-                missing_decl = (env1.missing_decl)
+                missing_decl = (env1.missing_decl);
+                pending_lemmas = (env1.pending_lemmas)
               })
          | FStar_Pervasives_Native.Some (uu___1, m) ->
              let next = m + Prims.int_one in
@@ -2572,7 +2792,8 @@ let (incr_query_index : env -> env) =
                 unif_allow_ref_guards = (env1.unif_allow_ref_guards);
                 erase_erasable_args = (env1.erase_erasable_args);
                 core_check = (env1.core_check);
-                missing_decl = (env1.missing_decl)
+                missing_decl = (env1.missing_decl);
+                pending_lemmas = (env1.pending_lemmas)
               }))
 let (set_range : env -> FStar_Compiler_Range_Type.range -> env) =
   fun e ->
@@ -2633,7 +2854,8 @@ let (set_range : env -> FStar_Compiler_Range_Type.range -> env) =
           unif_allow_ref_guards = (e.unif_allow_ref_guards);
           erase_erasable_args = (e.erase_erasable_args);
           core_check = (e.core_check);
-          missing_decl = (e.missing_decl)
+          missing_decl = (e.missing_decl);
+          pending_lemmas = (e.pending_lemmas)
         }
 let (get_range : env -> FStar_Compiler_Range_Type.range) = fun e -> e.range
 let (toggle_id_info : env -> Prims.bool -> unit) =
@@ -2732,7 +2954,8 @@ let (set_current_module : env -> FStar_Ident.lident -> env) =
         unif_allow_ref_guards = (env1.unif_allow_ref_guards);
         erase_erasable_args = (env1.erase_erasable_args);
         core_check = (env1.core_check);
-        missing_decl = (env1.missing_decl)
+        missing_decl = (env1.missing_decl);
+        pending_lemmas = (env1.pending_lemmas)
       }
 let (has_interface : env -> FStar_Ident.lident -> Prims.bool) =
   fun env1 ->
@@ -5395,11 +5618,34 @@ let (push_sigelt' : Prims.bool -> env -> FStar_Syntax_Syntax.sigelt -> env) =
             unif_allow_ref_guards = (env1.unif_allow_ref_guards);
             erase_erasable_args = (env1.erase_erasable_args);
             core_check = (env1.core_check);
-            missing_decl = (env1.missing_decl)
+            missing_decl = (env1.missing_decl);
+            pending_lemmas = (env1.pending_lemmas)
           } in
         add_sigelt force env2 s;
         (env2.tc_hooks).tc_push_in_gamma_hook env2 (FStar_Pervasives.Inr sb);
-        (let env3 = record_vals_and_defns env2 s in env3)
+        (let env3 = record_vals_and_defns env2 s in
+         match s.FStar_Syntax_Syntax.sigel with
+         | FStar_Syntax_Syntax.Sig_declare_typ
+             { FStar_Syntax_Syntax.lid2 = lid;
+               FStar_Syntax_Syntax.us2 = uu___2;
+               FStar_Syntax_Syntax.t2 = t;_}
+             -> maybe_add_pending_lemma env3 lid t
+         | FStar_Syntax_Syntax.Sig_let
+             { FStar_Syntax_Syntax.lbs1 = lbs;
+               FStar_Syntax_Syntax.lids1 = uu___2;_}
+             ->
+             FStar_Compiler_List.fold_left
+               (fun env4 ->
+                  fun lb ->
+                    let uu___3 =
+                      let uu___4 =
+                        FStar_Compiler_Util.right
+                          lb.FStar_Syntax_Syntax.lbname in
+                      FStar_Syntax_Syntax.lid_of_fv uu___4 in
+                    maybe_add_pending_lemma env4 uu___3
+                      lb.FStar_Syntax_Syntax.lbtyp) env3
+               (FStar_Pervasives_Native.snd lbs)
+         | uu___2 -> env3)
 let (push_sigelt : env -> FStar_Syntax_Syntax.sigelt -> env) =
   push_sigelt' false
 let (push_sigelt_force : env -> FStar_Syntax_Syntax.sigelt -> env) =
@@ -5476,7 +5722,8 @@ let (push_new_effect :
             unif_allow_ref_guards = (env1.unif_allow_ref_guards);
             erase_erasable_args = (env1.erase_erasable_args);
             core_check = (env1.core_check);
-            missing_decl = (env1.missing_decl)
+            missing_decl = (env1.missing_decl);
+            pending_lemmas = (env1.pending_lemmas)
           }
 let (exists_polymonadic_bind :
   env ->
@@ -5900,7 +6147,8 @@ let (update_effect_lattice :
              unif_allow_ref_guards = (env1.unif_allow_ref_guards);
              erase_erasable_args = (env1.erase_erasable_args);
              core_check = (env1.core_check);
-             missing_decl = (env1.missing_decl)
+             missing_decl = (env1.missing_decl);
+             pending_lemmas = (env1.pending_lemmas)
            })
 let (add_polymonadic_bind :
   env ->
@@ -5974,7 +6222,8 @@ let (add_polymonadic_bind :
               unif_allow_ref_guards = (env1.unif_allow_ref_guards);
               erase_erasable_args = (env1.erase_erasable_args);
               core_check = (env1.core_check);
-              missing_decl = (env1.missing_decl)
+              missing_decl = (env1.missing_decl);
+              pending_lemmas = (env1.pending_lemmas)
             }
 let (add_polymonadic_subcomp :
   env ->
@@ -6051,7 +6300,8 @@ let (add_polymonadic_subcomp :
                 unif_allow_ref_guards = (env1.unif_allow_ref_guards);
                 erase_erasable_args = (env1.erase_erasable_args);
                 core_check = (env1.core_check);
-                missing_decl = (env1.missing_decl)
+                missing_decl = (env1.missing_decl);
+                pending_lemmas = (env1.pending_lemmas)
               }
 let (push_local_binding : env -> FStar_Syntax_Syntax.binding -> env) =
   fun env1 ->
@@ -6109,7 +6359,8 @@ let (push_local_binding : env -> FStar_Syntax_Syntax.binding -> env) =
         unif_allow_ref_guards = (env1.unif_allow_ref_guards);
         erase_erasable_args = (env1.erase_erasable_args);
         core_check = (env1.core_check);
-        missing_decl = (env1.missing_decl)
+        missing_decl = (env1.missing_decl);
+        pending_lemmas = (env1.pending_lemmas)
       }
 let (push_bv : env -> FStar_Syntax_Syntax.bv -> env) =
   fun env1 ->
@@ -6179,7 +6430,8 @@ let (pop_bv :
               unif_allow_ref_guards = (env1.unif_allow_ref_guards);
               erase_erasable_args = (env1.erase_erasable_args);
               core_check = (env1.core_check);
-              missing_decl = (env1.missing_decl)
+              missing_decl = (env1.missing_decl);
+              pending_lemmas = (env1.pending_lemmas)
             })
     | uu___ -> FStar_Pervasives_Native.None
 let (push_binders : env -> FStar_Syntax_Syntax.binders -> env) =
@@ -6293,7 +6545,8 @@ let (set_expected_typ : env -> FStar_Syntax_Syntax.typ -> env) =
         unif_allow_ref_guards = (env1.unif_allow_ref_guards);
         erase_erasable_args = (env1.erase_erasable_args);
         core_check = (env1.core_check);
-        missing_decl = (env1.missing_decl)
+        missing_decl = (env1.missing_decl);
+        pending_lemmas = (env1.pending_lemmas)
       }
 let (set_expected_typ_maybe_eq :
   env -> FStar_Syntax_Syntax.typ -> Prims.bool -> env) =
@@ -6353,7 +6606,8 @@ let (set_expected_typ_maybe_eq :
           unif_allow_ref_guards = (env1.unif_allow_ref_guards);
           erase_erasable_args = (env1.erase_erasable_args);
           core_check = (env1.core_check);
-          missing_decl = (env1.missing_decl)
+          missing_decl = (env1.missing_decl);
+          pending_lemmas = (env1.pending_lemmas)
         }
 let (expected_typ :
   env ->
@@ -6423,7 +6677,8 @@ let (clear_expected_typ :
        unif_allow_ref_guards = (env_.unif_allow_ref_guards);
        erase_erasable_args = (env_.erase_erasable_args);
        core_check = (env_.core_check);
-       missing_decl = (env_.missing_decl)
+       missing_decl = (env_.missing_decl);
+       pending_lemmas = (env_.pending_lemmas)
      }, uu___)
 let (finish_module : env -> FStar_Syntax_Syntax.modul -> env) =
   let empty_lid =
@@ -6495,7 +6750,8 @@ let (finish_module : env -> FStar_Syntax_Syntax.modul -> env) =
         unif_allow_ref_guards = (env1.unif_allow_ref_guards);
         erase_erasable_args = (env1.erase_erasable_args);
         core_check = (env1.core_check);
-        missing_decl = (env1.missing_decl)
+        missing_decl = (env1.missing_decl);
+        pending_lemmas = (env1.pending_lemmas)
       }
 let (uvars_in_env : env -> FStar_Syntax_Syntax.uvars) =
   fun env1 ->
@@ -6707,7 +6963,8 @@ let (cons_proof_ns : Prims.bool -> env -> name_prefix -> env) =
           unif_allow_ref_guards = (e.unif_allow_ref_guards);
           erase_erasable_args = (e.erase_erasable_args);
           core_check = (e.core_check);
-          missing_decl = (e.missing_decl)
+          missing_decl = (e.missing_decl);
+          pending_lemmas = (e.pending_lemmas)
         }
 let (add_proof_ns : env -> name_prefix -> env) =
   fun e -> fun path -> cons_proof_ns true e path
@@ -6770,7 +7027,8 @@ let (set_proof_ns : proof_namespace -> env -> env) =
         unif_allow_ref_guards = (e.unif_allow_ref_guards);
         erase_erasable_args = (e.erase_erasable_args);
         core_check = (e.core_check);
-        missing_decl = (e.missing_decl)
+        missing_decl = (e.missing_decl);
+        pending_lemmas = (e.pending_lemmas)
       }
 let (unbound_vars :
   env ->
