ocaml/fstar-lib/generated/FStar_TypeChecker_Normalize.ml
@@ -8841,7 +8841,9 @@ let (eta_expand :
                                   FStar_TypeChecker_Env.core_check =
                                     (env1.FStar_TypeChecker_Env.core_check);
                                   FStar_TypeChecker_Env.missing_decl =
-                                    (env1.FStar_TypeChecker_Env.missing_decl)
+                                    (env1.FStar_TypeChecker_Env.missing_decl);
+                                  FStar_TypeChecker_Env.pending_lemmas =
+                                    (env1.FStar_TypeChecker_Env.pending_lemmas)
                                 } t true in
                             match uu___5 with
                             | (uu___6, ty, uu___7) ->
@@ -8953,7 +8955,9 @@ let (eta_expand :
                           FStar_TypeChecker_Env.core_check =
                             (env1.FStar_TypeChecker_Env.core_check);
                           FStar_TypeChecker_Env.missing_decl =
-                            (env1.FStar_TypeChecker_Env.missing_decl)
+                            (env1.FStar_TypeChecker_Env.missing_decl);
+                          FStar_TypeChecker_Env.pending_lemmas =
+                            (env1.FStar_TypeChecker_Env.pending_lemmas)
                         } t true in
                     (match uu___4 with
                      | (uu___5, ty, uu___6) -> eta_expand_with_type env1 t ty)))
