ocaml/fstar-lib/generated/FStar_TypeChecker_TcTerm.ml
@@ -100,7 +100,9 @@ let (instantiate_both :
       FStar_TypeChecker_Env.core_check =
         (env.FStar_TypeChecker_Env.core_check);
       FStar_TypeChecker_Env.missing_decl =
-        (env.FStar_TypeChecker_Env.missing_decl)
+        (env.FStar_TypeChecker_Env.missing_decl);
+      FStar_TypeChecker_Env.pending_lemmas =
+        (env.FStar_TypeChecker_Env.pending_lemmas)
     }
 let (no_inst : FStar_TypeChecker_Env.env -> FStar_TypeChecker_Env.env) =
   fun env ->
@@ -184,7 +186,9 @@ let (no_inst : FStar_TypeChecker_Env.env -> FStar_TypeChecker_Env.env) =
       FStar_TypeChecker_Env.core_check =
         (env.FStar_TypeChecker_Env.core_check);
       FStar_TypeChecker_Env.missing_decl =
-        (env.FStar_TypeChecker_Env.missing_decl)
+        (env.FStar_TypeChecker_Env.missing_decl);
+      FStar_TypeChecker_Env.pending_lemmas =
+        (env.FStar_TypeChecker_Env.pending_lemmas)
     }
 let (is_eq :
   FStar_Syntax_Syntax.binder_qualifier FStar_Pervasives_Native.option ->
@@ -1298,7 +1302,9 @@ let (guard_letrecs :
                 FStar_TypeChecker_Env.core_check =
                   (env.FStar_TypeChecker_Env.core_check);
                 FStar_TypeChecker_Env.missing_decl =
-                  (env.FStar_TypeChecker_Env.missing_decl)
+                  (env.FStar_TypeChecker_Env.missing_decl);
+                FStar_TypeChecker_Env.pending_lemmas =
+                  (env.FStar_TypeChecker_Env.pending_lemmas)
               } in
             let decreases_clause bs c =
               (let uu___1 = FStar_Compiler_Debug.low () in
@@ -1953,7 +1959,9 @@ let rec (tc_term :
                   FStar_TypeChecker_Env.core_check =
                     (env.FStar_TypeChecker_Env.core_check);
                   FStar_TypeChecker_Env.missing_decl =
-                    (env.FStar_TypeChecker_Env.missing_decl)
+                    (env.FStar_TypeChecker_Env.missing_decl);
+                  FStar_TypeChecker_Env.pending_lemmas =
+                    (env.FStar_TypeChecker_Env.pending_lemmas)
                 } e) in
        match uu___2 with
        | (r, ms) ->
@@ -2276,7 +2284,9 @@ and (tc_maybe_toplevel_term :
                           FStar_TypeChecker_Env.core_check =
                             (env'.FStar_TypeChecker_Env.core_check);
                           FStar_TypeChecker_Env.missing_decl =
-                            (env'.FStar_TypeChecker_Env.missing_decl)
+                            (env'.FStar_TypeChecker_Env.missing_decl);
+                          FStar_TypeChecker_Env.pending_lemmas =
+                            (env'.FStar_TypeChecker_Env.pending_lemmas)
                         } in
                       let uu___4 = tc_term env'1 qt in
                       (match uu___4 with
@@ -4545,7 +4555,9 @@ and (tc_tactic :
               FStar_TypeChecker_Env.core_check =
                 (env.FStar_TypeChecker_Env.core_check);
               FStar_TypeChecker_Env.missing_decl =
-                (env.FStar_TypeChecker_Env.missing_decl)
+                (env.FStar_TypeChecker_Env.missing_decl);
+              FStar_TypeChecker_Env.pending_lemmas =
+                (env.FStar_TypeChecker_Env.pending_lemmas)
             } in
           let uu___ = FStar_Syntax_Syntax.t_tac_of a b in
           tc_check_tot_or_gtot_term env1 tau uu___ ""
@@ -5246,7 +5258,9 @@ and (tc_comp :
                 FStar_TypeChecker_Env.core_check =
                   (env.FStar_TypeChecker_Env.core_check);
                 FStar_TypeChecker_Env.missing_decl =
-                  (env.FStar_TypeChecker_Env.missing_decl)
+                  (env.FStar_TypeChecker_Env.missing_decl);
+                FStar_TypeChecker_Env.pending_lemmas =
+                  (env.FStar_TypeChecker_Env.pending_lemmas)
               } tc FStar_Syntax_Syntax.teff "" in
           (match uu___ with
            | (tc1, uu___1, f) ->
@@ -5749,7 +5763,9 @@ and (tc_abs_expected_function_typ :
                                FStar_TypeChecker_Env.core_check =
                                  (envbody.FStar_TypeChecker_Env.core_check);
                                FStar_TypeChecker_Env.missing_decl =
-                                 (envbody.FStar_TypeChecker_Env.missing_decl)
+                                 (envbody.FStar_TypeChecker_Env.missing_decl);
+                               FStar_TypeChecker_Env.pending_lemmas =
+                                 (envbody.FStar_TypeChecker_Env.pending_lemmas)
                              } in
                            let uu___2 =
                              FStar_Compiler_List.fold_left
@@ -5905,7 +5921,9 @@ and (tc_abs_expected_function_typ :
                              FStar_TypeChecker_Env.core_check =
                                (env.FStar_TypeChecker_Env.core_check);
                              FStar_TypeChecker_Env.missing_decl =
-                               (env.FStar_TypeChecker_Env.missing_decl)
+                               (env.FStar_TypeChecker_Env.missing_decl);
+                             FStar_TypeChecker_Env.pending_lemmas =
+                               (env.FStar_TypeChecker_Env.pending_lemmas)
                            } in
                          let uu___2 =
                            check_actuals_against_formals envbody bs
@@ -6022,7 +6040,9 @@ and (tc_abs_expected_function_typ :
                                   FStar_TypeChecker_Env.core_check =
                                     (envbody1.FStar_TypeChecker_Env.core_check);
                                   FStar_TypeChecker_Env.missing_decl =
-                                    (envbody1.FStar_TypeChecker_Env.missing_decl)
+                                    (envbody1.FStar_TypeChecker_Env.missing_decl);
+                                  FStar_TypeChecker_Env.pending_lemmas =
+                                    (envbody1.FStar_TypeChecker_Env.pending_lemmas)
                                 } in
                               let uu___3 = mk_letrec_env envbody2 bs1 c in
                               (match uu___3 with
@@ -6640,7 +6660,9 @@ and (tc_abs :
                                   FStar_TypeChecker_Env.core_check =
                                     (envbody2.FStar_TypeChecker_Env.core_check);
                                   FStar_TypeChecker_Env.missing_decl =
-                                    (envbody2.FStar_TypeChecker_Env.missing_decl)
+                                    (envbody2.FStar_TypeChecker_Env.missing_decl);
+                                  FStar_TypeChecker_Env.pending_lemmas =
+                                    (envbody2.FStar_TypeChecker_Env.pending_lemmas)
                                 } body2 in
                             (match uu___7 with
                              | (body3, cbody, guard_body) ->
@@ -10322,7 +10344,10 @@ and (tc_eqn :
                                                                     (uu___16.FStar_TypeChecker_Env.core_check);
                                                                     FStar_TypeChecker_Env.missing_decl
                                                                     =
-                                                                    (uu___16.FStar_TypeChecker_Env.missing_decl)
+                                                                    (uu___16.FStar_TypeChecker_Env.missing_decl);
+                                                                    FStar_TypeChecker_Env.pending_lemmas
+                                                                    =
+                                                                    (uu___16.FStar_TypeChecker_Env.pending_lemmas)
                                                                     } in
                                                                    let uu___16
                                                                     =
@@ -10807,7 +10832,9 @@ and (check_inner_let :
               FStar_TypeChecker_Env.core_check =
                 (env1.FStar_TypeChecker_Env.core_check);
               FStar_TypeChecker_Env.missing_decl =
-                (env1.FStar_TypeChecker_Env.missing_decl)
+                (env1.FStar_TypeChecker_Env.missing_decl);
+              FStar_TypeChecker_Env.pending_lemmas =
+                (env1.FStar_TypeChecker_Env.pending_lemmas)
             } in
           let uu___ =
             let uu___1 =
@@ -11592,7 +11619,9 @@ and (build_let_rec_env :
                 FStar_TypeChecker_Env.core_check =
                   (env01.FStar_TypeChecker_Env.core_check);
                 FStar_TypeChecker_Env.missing_decl =
-                  (env01.FStar_TypeChecker_Env.missing_decl)
+                  (env01.FStar_TypeChecker_Env.missing_decl);
+                FStar_TypeChecker_Env.pending_lemmas =
+                  (env01.FStar_TypeChecker_Env.pending_lemmas)
               } t uu___1 "" in
           match uu___ with
           | (t1, uu___1, g) ->
@@ -11798,7 +11827,10 @@ and (build_let_rec_env :
                                              (env2.FStar_TypeChecker_Env.core_check);
                                            FStar_TypeChecker_Env.missing_decl
                                              =
-                                             (env2.FStar_TypeChecker_Env.missing_decl)
+                                             (env2.FStar_TypeChecker_Env.missing_decl);
+                                           FStar_TypeChecker_Env.pending_lemmas
+                                             =
+                                             (env2.FStar_TypeChecker_Env.pending_lemmas)
                                          } in
                                        (lb1, env3)))
                                  | FStar_Pervasives_Native.None ->
@@ -12080,7 +12112,9 @@ and (check_let_bound_def :
                          FStar_TypeChecker_Env.core_check =
                            (env11.FStar_TypeChecker_Env.core_check);
                          FStar_TypeChecker_Env.missing_decl =
-                           (env11.FStar_TypeChecker_Env.missing_decl)
+                           (env11.FStar_TypeChecker_Env.missing_decl);
+                         FStar_TypeChecker_Env.pending_lemmas =
+                           (env11.FStar_TypeChecker_Env.pending_lemmas)
                        } e11 in
                    match uu___4 with
                    | (e12, c1, g1) ->
@@ -12602,7 +12636,9 @@ let (typeof_tot_or_gtot_term :
              FStar_TypeChecker_Env.core_check =
                (env.FStar_TypeChecker_Env.core_check);
              FStar_TypeChecker_Env.missing_decl =
-               (env.FStar_TypeChecker_Env.missing_decl)
+               (env.FStar_TypeChecker_Env.missing_decl);
+             FStar_TypeChecker_Env.pending_lemmas =
+               (env.FStar_TypeChecker_Env.pending_lemmas)
            } in
          let uu___1 =
            try
@@ -12792,7 +12828,9 @@ let (level_of_type :
                          FStar_TypeChecker_Env.core_check =
                            (env.FStar_TypeChecker_Env.core_check);
                          FStar_TypeChecker_Env.missing_decl =
-                           (env.FStar_TypeChecker_Env.missing_decl)
+                           (env.FStar_TypeChecker_Env.missing_decl);
+                         FStar_TypeChecker_Env.pending_lemmas =
+                           (env.FStar_TypeChecker_Env.pending_lemmas)
                        } in
                      let g = FStar_TypeChecker_Rel.teq env1 t1 t_u in
                      ((match g.FStar_TypeChecker_Common.guard_f with
@@ -13205,7 +13243,9 @@ let rec (universe_of_aux :
                          FStar_TypeChecker_Env.core_check =
                            (env2.FStar_TypeChecker_Env.core_check);
                          FStar_TypeChecker_Env.missing_decl =
-                           (env2.FStar_TypeChecker_Env.missing_decl)
+                           (env2.FStar_TypeChecker_Env.missing_decl);
+                         FStar_TypeChecker_Env.pending_lemmas =
+                           (env2.FStar_TypeChecker_Env.pending_lemmas)
                        } in
                      ((let uu___5 =
                          FStar_Compiler_Effect.op_Bang dbg_UniverseOf in
