ocaml/fstar-lib/generated/FStar_TypeChecker_Util.ml
@@ -5679,7 +5679,10 @@ let (find_coercion :
                                                                     (env.FStar_TypeChecker_Env.core_check);
                                                                     FStar_TypeChecker_Env.missing_decl
                                                                     =
-                                                                    (env.FStar_TypeChecker_Env.missing_decl)
+                                                                    (env.FStar_TypeChecker_Env.missing_decl);
+                                                                    FStar_TypeChecker_Env.pending_lemmas
+                                                                    =
+                                                                    (env.FStar_TypeChecker_Env.pending_lemmas)
                                                                     } tt in
                                                                     FStar_Pervasives_Native.Some
                                                                     uu___21)))))))))
@@ -8098,7 +8101,9 @@ let (update_env_sub_eff :
               FStar_TypeChecker_Env.core_check =
                 (env.FStar_TypeChecker_Env.core_check);
               FStar_TypeChecker_Env.missing_decl =
-                (env.FStar_TypeChecker_Env.missing_decl)
+                (env.FStar_TypeChecker_Env.missing_decl);
+              FStar_TypeChecker_Env.pending_lemmas =
+                (env.FStar_TypeChecker_Env.pending_lemmas)
             } sub.FStar_Syntax_Syntax.source sub.FStar_Syntax_Syntax.target
             uu___ in
         {
@@ -8196,7 +8201,9 @@ let (update_env_sub_eff :
           FStar_TypeChecker_Env.core_check =
             (env1.FStar_TypeChecker_Env.core_check);
           FStar_TypeChecker_Env.missing_decl =
-            (env1.FStar_TypeChecker_Env.missing_decl)
+            (env1.FStar_TypeChecker_Env.missing_decl);
+          FStar_TypeChecker_Env.pending_lemmas =
+            (env1.FStar_TypeChecker_Env.pending_lemmas)
         }
 let (update_env_polymonadic_bind :
   FStar_TypeChecker_Env.env ->
