ocaml/fstar-lib/generated/FStar_Universal.ml
@@ -117,7 +117,9 @@ let with_dsenv_of_tcenv :
               FStar_TypeChecker_Env.core_check =
                 (tcenv.FStar_TypeChecker_Env.core_check);
               FStar_TypeChecker_Env.missing_decl =
-                (tcenv.FStar_TypeChecker_Env.missing_decl)
+                (tcenv.FStar_TypeChecker_Env.missing_decl);
+              FStar_TypeChecker_Env.pending_lemmas =
+                (tcenv.FStar_TypeChecker_Env.pending_lemmas)
             })
 let with_tcenv_of_env :
   'a .
@@ -368,7 +370,9 @@ let (init_env : FStar_Parser_Dep.deps -> FStar_TypeChecker_Env.env) =
         FStar_TypeChecker_Env.core_check =
           (env.FStar_TypeChecker_Env.core_check);
         FStar_TypeChecker_Env.missing_decl =
-          (env.FStar_TypeChecker_Env.missing_decl)
+          (env.FStar_TypeChecker_Env.missing_decl);
+        FStar_TypeChecker_Env.pending_lemmas =
+          (env.FStar_TypeChecker_Env.pending_lemmas)
       } in
     let env2 =
       {
@@ -461,7 +465,9 @@ let (init_env : FStar_Parser_Dep.deps -> FStar_TypeChecker_Env.env) =
         FStar_TypeChecker_Env.core_check =
           (env1.FStar_TypeChecker_Env.core_check);
         FStar_TypeChecker_Env.missing_decl =
-          (env1.FStar_TypeChecker_Env.missing_decl)
+          (env1.FStar_TypeChecker_Env.missing_decl);
+        FStar_TypeChecker_Env.pending_lemmas =
+          (env1.FStar_TypeChecker_Env.pending_lemmas)
       } in
     let env3 =
       {
@@ -554,7 +560,9 @@ let (init_env : FStar_Parser_Dep.deps -> FStar_TypeChecker_Env.env) =
         FStar_TypeChecker_Env.core_check =
           (env2.FStar_TypeChecker_Env.core_check);
         FStar_TypeChecker_Env.missing_decl =
-          (env2.FStar_TypeChecker_Env.missing_decl)
+          (env2.FStar_TypeChecker_Env.missing_decl);
+        FStar_TypeChecker_Env.pending_lemmas =
+          (env2.FStar_TypeChecker_Env.pending_lemmas)
       } in
     let env4 =
       {
@@ -646,7 +654,9 @@ let (init_env : FStar_Parser_Dep.deps -> FStar_TypeChecker_Env.env) =
         FStar_TypeChecker_Env.core_check =
           (env3.FStar_TypeChecker_Env.core_check);
         FStar_TypeChecker_Env.missing_decl =
-          (env3.FStar_TypeChecker_Env.missing_decl)
+          (env3.FStar_TypeChecker_Env.missing_decl);
+        FStar_TypeChecker_Env.pending_lemmas =
+          (env3.FStar_TypeChecker_Env.pending_lemmas)
       } in
     let env5 =
       {
@@ -738,7 +748,9 @@ let (init_env : FStar_Parser_Dep.deps -> FStar_TypeChecker_Env.env) =
         FStar_TypeChecker_Env.core_check =
           (env4.FStar_TypeChecker_Env.core_check);
         FStar_TypeChecker_Env.missing_decl =
-          (env4.FStar_TypeChecker_Env.missing_decl)
+          (env4.FStar_TypeChecker_Env.missing_decl);
+        FStar_TypeChecker_Env.pending_lemmas =
+          (env4.FStar_TypeChecker_Env.pending_lemmas)
       } in
     (env5.FStar_TypeChecker_Env.solver).FStar_TypeChecker_Env.init env5; env5
 type lang_decls_t = FStar_Parser_AST.decl Prims.list
