src/typechecker/FStar.TypeChecker.ContextPruning.fst
@@ -1,0 +1,133 @@
+module FStar.TypeChecker.ContextPruning
+open FStar.Compiler
+open FStar.Compiler.Effect
+open FStar.Ident
+open FStar.Syntax.Syntax
+open FStar.TypeChecker.Env
+open FStar.Class.Monad
+module BU = FStar.Compiler.Util
+module SS = FStar.Syntax.Subst
+open FStar.Class.Setlike
+
+type ctxt = {
+  env: env;
+  reached: list lident;
+  pending_lemmas: pending_lemma_patterns;
+}
+
+
+let st a = ctxt -> (a & ctxt)
+let get : st ctxt = fun s -> (s, s)
+let put (c:ctxt) : st unit = fun _ -> ((), c)
+instance st_monad: monad st = {
+  return= (fun (#a:Type) (x:a) -> (fun s -> (x, s)) <: st a);
+  ( let! ) = (fun (#a #b:Type) (m:st a) (f:a -> st b) (s:ctxt) ->
+                let (x, s) = m s in
+                f x s)
+}
+
+let remove_trigger (lid:lident)
+: st unit
+= let! ctxt = get in
+  put {ctxt with pending_lemmas=remove_pending_lemma lid ctxt.pending_lemmas}
+
+let find_lemmas_waiting_on_trigger (lid:lident)
+: st (list lident)
+= let! ctxt = get in
+  return <| Env.find_lemmas_waiting_on_trigger lid ctxt.pending_lemmas
+
+let remove_trigger_for_lemma (pat:lident) (lem:lident)
+: st bool
+= let! ctxt = get in
+  let pp, eligible = Env.remove_trigger_for_lemma pat lem ctxt.pending_lemmas in
+  put {ctxt with pending_lemmas=pp} ;!
+  return eligible
+ 
+let ctx_contains (x:lident)
+: st bool
+= let! ctxt = get in
+  return (List.mem x ctxt.reached)
+
+let lookup_definition (x:lident)
+: st (option (univ_names & term))
+= let! ctxt = get in
+  return <| FStar.TypeChecker.Env.lookup_definition [Env.Unfold delta_constant] ctxt.env x
+let lookup_type (x:lident)
+: st (option (univ_names & term))
+= return None
+let add_lident (x:lident)
+: st unit
+= let! ctxt = get in
+  put {ctxt with reached=x::ctxt.reached}
+
+let rec context_of_term (t:term)
+: st (list lident)
+= let fvs = FStar.Syntax.Free.fvars t in
+  foldM_left
+    (fun acc fv ->
+      if! ctx_contains fv
+      then return acc
+      else (
+        add_lident fv ;!
+        match! lookup_definition fv with
+        | None -> return (fv::acc)
+        | Some (_, t) -> let! fvs = context_of_term t in return (fv::fvs)))
+    []
+    (elems fvs)
+
+let trigger_pending_lemmas (lids:list lident)
+: st (either (list lident) bool) //either some lemmas were triggered; or maybe nothing changed
+= foldM_left
+    (fun acc lid ->
+      match! find_lemmas_waiting_on_trigger lid with
+      | [] -> return acc
+      | lemmas ->
+        remove_trigger lid ;!
+        let! eligible_lemmas =
+          foldM_left
+            (fun acc lem ->
+              if! remove_trigger_for_lemma lid lem
+              then return (lem::acc)
+              else return acc)
+            []
+            lemmas
+        in
+        match eligible_lemmas with
+        | [] -> return (Inr true) //something changed
+        | _ -> return (Inl eligible_lemmas))
+  (Inr false)
+  lids
+open FStar.List.Tot
+let rec scan (ts:list term)
+: st unit
+= let! new_fvs =
+    foldM_left
+      (fun acc t ->
+        let! new_fvs = context_of_term t in
+        return (new_fvs @ acc))
+      [] ts
+  in
+  match! trigger_pending_lemmas new_fvs with
+  | Inl triggered ->
+    let! lemma_types =
+      foldM_left
+        (fun acc lem ->
+          if! ctx_contains lem
+          then return acc
+          else (
+            add_lident lem ;!
+            match! lookup_type lem with
+            | None -> return acc
+            | Some (_, t) -> return (t::acc)
+          ))
+        []
+        triggered
+    in
+    scan lemma_types
+  | Inr _ -> return ()
+
+let context_of (env:env) (t:term)
+: list lident
+= let init = { env; pending_lemmas=env.pending_lemmas; reached=[] } in
+  let _, ctxt = scan [t] init in
+  ctxt.reached
