src/typechecker/FStar.TypeChecker.ContextPruning.fsti
@@ -1,0 +1,5 @@
+module FStar.TypeChecker.ContextPruning
+open FStar.Syntax.Syntax
+open FStar.TypeChecker.Env
+open FStar.Ident
+val context_of (env:env) (t:term) : list lident
